feat: add new typing rules

CollapsingTowers/TwoLevelPCP/Typing.lean
@@ -3,8 +3,60 @@ import CollapsingTowers.TwoLevelPCP.Syntax
 import CollapsingTowers.TwoLevelPCP.SmallStep
 import CollapsingTowers.TwoLevelPCP.Env
 inductive typing : Stage → TEnv → Expr → Ty → Prop where
-  | fvar : ∀ 𝕊 Γ x τ, binds x τ 𝕊 Γ -> typing 𝕊 Γ (.fvar x) τ
+  | fvar : ∀ 𝕊 Γ x τ,
+    binds x τ 𝕊 Γ ->
+    typing 𝕊 Γ (.fvar x) τ
   | lam₁ : ∀ 𝕊 Γ e τ𝕒 τ𝕓,
     typing 𝕊 ((τ𝕒, 𝕊) :: Γ) (open₀ Γ.length e) τ𝕓 ->
     closed_at e Γ.length ->
     typing 𝕊 Γ (.lam₁ e) (.arrow τ𝕒 τ𝕓)
+  | lift_lam : ∀ Γ e τ𝕒 τ𝕓,
+    typing .fst Γ e (.arrow (.rep₁ τ𝕒) (.rep₁ τ𝕓)) ->
+    typing .fst Γ (.lift e) (.rep₁ (.arrow τ𝕒 τ𝕓))
+  | app₁ : ∀ 𝕊 Γ f arg τ𝕒 τ𝕓,
+    typing 𝕊 Γ f (.arrow τ𝕒 τ𝕓) ->
+    typing 𝕊 Γ arg τ𝕒 ->
+    typing 𝕊 Γ (.app₁ f arg) τ𝕓
+  | app₂ : ∀ Γ f arg τ𝕒 τ𝕓,
+    typing .fst Γ f (.rep₁ (.arrow τ𝕒 τ𝕓)) ->
+    typing .fst Γ arg (.rep₁ τ𝕒) ->
+    typing .fst Γ (.app₂ f arg) (.rep₁ τ𝕓)
+  | plus₁ : ∀ 𝕊 Γ l r,
+    typing 𝕊 Γ l .nat ->
+    typing 𝕊 Γ r .nat ->
+    typing 𝕊 Γ (.plus₁ l r) .nat
+  | plus₂ : ∀ Γ l r,
+    typing .fst Γ l (.rep₁ .nat) ->
+    typing .fst Γ r (.rep₁ .nat) ->
+    typing .fst Γ (.plus₂ l r) (.rep₁ .nat)
+  | lit₁ : ∀ 𝕊 Γ n,
+    typing 𝕊 Γ (.lit₁ n) .nat
+  | lift_lit : ∀ Γ n,
+    typing .fst Γ n .nat ->
+    typing .fst Γ (.lift n) (.rep₁ .nat)
+  | code₁ : ∀ Γ x τ,
+    binds x τ .snd Γ ->
+    typing .fst Γ (.code (.fvar x)) (.rep₁ τ)
+  | code₂ : ∀ Γ e τ,
+    typing .snd Γ e τ ->
+    typing .snd Γ (.code e) (.rep₂ τ)
+  | lift_code : ∀ Γ e τ,
+    typing .fst Γ e (.rep₁ τ) ->
+    typing .snd Γ e (.rep₂ τ)
+  | reflect : ∀ Γ e τ,
+    typing .snd Γ e τ ->
+    typing .fst Γ (.reflect e) (.rep₁ τ)
+  | lam𝕔 : ∀ Γ e τ𝕒 τ𝕓,
+    typing .snd ((τ𝕒, .snd) :: Γ) (open₀ Γ.length e) (.rep₂ τ𝕓) ->
+    closed_at e Γ.length ->
+    typing .fst Γ (.lam𝕔 e) (.rep₁ (.arrow τ𝕒 τ𝕓))
+  | lets : ∀ 𝕊 Γ b e τ𝕒 τ𝕓,
+    typing 𝕊 Γ b τ𝕒 ->
+    typing 𝕊 ((τ𝕒, 𝕊) :: Γ) (open₀ Γ.length e) τ𝕓 ->
+    closed_at e Γ.length ->
+    typing 𝕊 Γ (.lets b e) τ𝕓
+  | let𝕔 : ∀ Γ b e τ𝕒 τ𝕓,
+    typing .snd Γ b τ𝕒 ->
+    typing .snd ((τ𝕒, .snd) :: Γ) (open₀ Γ.length e) (.rep₂ τ𝕓) ->
+    closed_at e Γ.length ->
+    typing .snd Γ (.let𝕔 b e) (.rep₂ τ𝕓)
