CollapsingTowers/TwoLevelPCP/Example.lean
@@ -1,0 +1,128 @@
+
+import Mathlib.Data.Finset.Basic
+import CollapsingTowers.TwoLevelPCP.SmallStep
+import CollapsingTowers.TwoLevelPCP.Typing
+namespace Example1
+
+/-- Example 1:
+lift x. x +₂ (x +₂ x)
+→⋆
+code {
+  lets f = lam₁ x.
+    lets y = x + x in
+    lets z = x + y in z
+  in f
+}
+-/
+def x₀ : Expr :=
+  .fvar 0
+
+def x₁ : Expr :=
+  .fvar 1
+
+def x₂ : Expr :=
+  .fvar 2
+
+def x₃ : Expr :=
+  .fvar 3
+
+def expr₀ : Expr :=
+  .lift (.lam₁ (close₀ 0 (.plus₂ x₀ (.plus₂ x₀ x₀))))
+
+def expr₁ : Expr :=
+  .lam𝕔 (close₀ 0 (.plus₂ (.code x₀) (.plus₂ (.code x₀) (.code x₀))))
+
+def expr₂ : Expr :=
+  .lam𝕔 (close₀ 0 (.plus₂ (.code x₀) (.reflect (.plus₁ x₀ x₀))))
+
+def expr₃ : Expr :=
+  .lam𝕔 (close₀ 0 (.let𝕔 (.plus₁ x₀ x₀) (close₀ 1 (.plus₂ (.code x₀) (.code x₁)))))
+
+def expr₄ : Expr :=
+  .lam𝕔 (close₀ 0 (.let𝕔 (.plus₁ x₀ x₀) (close₀ 1 (.reflect (.plus₁ x₀ x₁)))))
+
+def expr₅ : Expr :=
+  .lam𝕔 (close₀ 0 (.let𝕔 (.plus₁ x₀ x₀) (close₀ 1 (.let𝕔 (.plus₁ x₀ x₁) (close₀ 2 (.code x₂))))))
+
+def expr₆ : Expr :=
+  .lam𝕔 (close₀ 0 (.let𝕔 (.plus₁ x₀ x₀) (close₀ 1 (.code (.lets (.plus₁ x₀ x₁) (close₀ 2 x₂))))))
+
+def expr₇ : Expr :=
+  .lam𝕔 (close₀ 0 (.code (.lets (.plus₁ x₀ x₀) (close₀ 1 (.lets (.plus₁ x₀ x₁) (close₀ 2 x₂))))))
+
+def expr₈ : Expr :=
+  .reflect (.lam₁ (close₀ 0 (.lets (.plus₁ x₀ x₀) (close₀ 1 (.lets (.plus₁ x₀ x₁) (close₀ 2 x₂))))))
+
+def expr₉ : Expr :=
+  .let𝕔 (.lam₁ (close₀ 0 (.lets (.plus₁ x₀ x₀) (close₀ 1 (.lets (.plus₁ x₀ x₁) (close₀ 2 x₂)))))) (close₀ 3 (.code x₃))
+
+def expr𝕩 : Expr :=
+  .code (.lets (.lam₁ (close₀ 0 (.lets (.plus₁ x₀ x₀) (close₀ 1 (.lets (.plus₁ x₀ x₁) (close₀ 2 x₂)))))) (close₀ 3 x₃))
+
+def ty : Ty :=
+  .rep₂ (.arrow .nat .nat)
+
+example : typing .snd [] expr₀ ty := by
+  rw [expr₀, x₀, ty]
+  repeat constructor
+
+example : typing .snd [] expr₁ ty := by
+  rw [expr₁, x₀, ty]
+  repeat constructor
+
+example : typing .snd [] expr₂ ty := by
+  rw [expr₂, x₀, ty]
+  repeat constructor
+
+example : typing .snd [] expr₃ ty := by
+  rw [expr₃, x₀, x₁, ty]
+  apply typing.lift_code
+  apply typing.lam𝕔
+  apply typing.let𝕔
+  repeat constructor
+
+example : typing .snd [] expr₄ ty := by
+  rw [expr₄, x₀, x₁, ty]
+  apply typing.lift_code
+  apply typing.lam𝕔
+  apply typing.let𝕔
+  repeat constructor
+
+example : typing .snd [] expr₅ ty := by
+  rw [expr₅, x₀, x₁, x₂, ty]
+  apply typing.lift_code
+  apply typing.lam𝕔
+  repeat
+    ( apply typing.let𝕔 _ _ _ .nat
+      apply typing.plus₁
+      apply typing.fvar; simp
+      apply typing.fvar; simp)
+  repeat constructor
+
+example : typing .snd [] expr₆ ty := by
+  rw [expr₆, x₀, x₁, x₂, ty]
+  apply typing.lift_code
+  apply typing.lam𝕔
+  apply typing.let𝕔
+  repeat constructor
+
+example : typing .snd [] expr₇ ty := by
+  rw [expr₇, x₀, x₁, x₂, ty]
+  repeat constructor
+
+example : typing .snd [] expr₈ ty := by
+  rw [expr₈, x₀, x₁, x₂, ty]
+  repeat constructor
+
+example : typing .snd [] expr₉ ty := by
+  rw [expr₉, x₀, x₁, x₂, ty]
+  apply typing.let𝕔 _ _ _ (.arrow .nat .nat)
+  repeat constructor
+
+example : typing .snd [] expr𝕩 ty := by
+  rw [expr𝕩, x₀, x₁, x₂, ty]
+  apply typing.code₂
+  apply typing.lets _ _ _ _ (.arrow .nat .nat)
+  repeat constructor
+
+end Example1
